Refinery/Term/Extrinsic/Refinement/Subst/Basic.lean
@@ -1,0 +1,151 @@
+import Refinery.Term.Extrinsic.Refinement.Uniform
+import Refinery.Term.Extrinsic.Subst.Basic
+
+namespace Refinery
+
+namespace Term
+
+--NOTE: since only pure substitutions are uniform, I believe pure substitutions can be proven
+-- congruent for any UWkCongr relation, so we should be fine here in terms of expressive power
+-- We should still do relD? quotienting? Maybe?
+
+variable {φ : Type u} {α : Type v} {ε : Type w} [S : Signature φ α ε]
+
+inductive DRWS.relD? (R : DRWS φ α)
+  : ∀{Γ} {a a' : Term φ (Ty α)} {v}, (Γ ⊢? a : v) → (Γ ⊢? a' : v) → Prop
+  | valid {Γ : Ctx? α} {a a'} (A q) {da : Γ ⊢ a : A} {da' : Γ ⊢ a' : A} (h : R.rel da da') (hq)
+    : relD? R (.valid A q da hq) (.valid A q da' hq)
+  | zero {Γ : Ctx? α} (a a') (A) (hΓ : Γ.del) : relD? R (.zero hΓ a A) (.zero hΓ a' A)
+
+inductive DRWS.relS (R : DRWS φ α) : ∀{Γ Δ : Ctx? α}, SubstDS φ Γ Δ → SubstDS φ Γ Δ → Prop
+  | nil {Γ : Ctx? α} (hΓ : Γ.del) : relS R (.nil hΓ) (.nil hΓ)
+  | cons {Γ Γl Γr Δ : Ctx? α}
+    (hΓ : Γ.SSplit Γl Γr)
+    {σ σ' : SubstDS φ Γl Δ} (hσ : R.relS σ σ')
+    {a a'} {da : Γr ⊢? a : v} {da' : Γr ⊢? a' : v}
+    (ha : R.relD? da da') : relS R (σ.cons hΓ da) (σ'.cons hΓ da')
+  -- TODO: do we add transitivity here, or will it make things more complex?
+  -- (note: transitivity allows for multi-splitting)
+
+theorem DRWS.rel.substD_of_subst {R : DRWS φ α}
+  {Γ Δ : Ctx? α} (σ : SubstDS φ Γ Δ) {A a b} {da : Δ ⊢ a : A} {db : Δ ⊢ b : A}
+  (h : R.rel (da.subst σ) (db.subst σ)) : R.rel (da.substD σ) (db.substD σ)
+  := h.of_cast_term
+
+theorem DRWS.rel.subst_of_substD {R : DRWS φ α}
+  {Γ Δ : Ctx? α} (σ : SubstDS φ Γ Δ) {A a b} {da : Δ ⊢ a : A} {db : Δ ⊢ b : A}
+  (h : R.rel (da.substD σ) (db.substD σ)) : R.rel (da.subst σ) (db.subst σ)
+  := h.cast_term _ _
+
+theorem DRWS.rel.substD_iff_subst {R : DRWS φ α}
+  {Γ Δ : Ctx? α} (σ : SubstDS φ Γ Δ) {A a b} {da : Δ ⊢ a : A} {db : Δ ⊢ b : A}
+  : R.rel (da.subst σ) (db.subst σ) ↔ R.rel (da.substD σ) (db.substD σ)
+  := ⟨DRWS.rel.substD_of_subst _, DRWS.rel.subst_of_substD _⟩
+
+class DRWS.SubstCongr (R : DRWS φ α) where
+  csubst_congr {Γ Δ : Ctx? α} (σ : SubstDS φ Γ Δ) {A a b} (da : Δ ⊢ a : A) (db : Δ ⊢ b : A) :
+    R.rel da db → R.cohere.rel (da.subst σ) (db.subst σ)
+
+instance DRWS.SubstCongr.instBot : SubstCongr (⊥ : DRWS φ α) where
+  csubst_congr _ _ _ _ _ _  h:= h.elim
+
+theorem DRWS.rel.csubst_congr [SubstCongr R]
+  {Γ Δ : Ctx? α} (σ : SubstDS φ Γ Δ) {A a b} {da : Δ ⊢ a : A} {db : Δ ⊢ b : A}
+  : R.rel da db → R.cohere.rel (da.subst σ) (db.subst σ)
+  := SubstCongr.csubst_congr σ da db
+
+instance DRWS.subst_congr_symm (R : DRWS φ α) [SubstCongr R] : R.symm.SubstCongr where
+  csubst_congr ρ _ _ _ _ _
+    | .fwd h => (h.csubst_congr ρ).mono R.symm_increasing
+    | .bwd h => (h.csubst_congr ρ).toSwap.toCohere.mono R.swap_le_symm
+
+class DRWS.USubstCongr (R : DRWS φ α) where
+  usubst_congr {Γ Δ : Ctx? α} (σ : SubstDS φ Γ Δ) {A a b} (da : Δ ⊢ a : A) (db : Δ ⊢ b : A) :
+    R.rel da db → R.uniform.rel (da.subst σ) (db.subst σ)
+
+instance DRWS.USubstCongr.of_subst_congr {R : DRWS φ α} [SubstCongr R] : USubstCongr R where
+  usubst_congr ρ _ _ _ _ _ h := R.uniform_le_cohere _ _ _ _ _ _ (h.csubst_congr ρ)
+
+theorem DRWS.rel.usubst_congr [USubstCongr R]
+  {Γ Δ : Ctx? α} (σ : SubstDS φ Γ Δ) {A a b} {da : Δ ⊢ a : A} {db : Δ ⊢ b : A}
+  : R.rel da db → R.uniform.rel (da.subst σ) (db.subst σ)
+  := USubstCongr.usubst_congr σ da db
+
+-- -- OOPS: only _pure_ substitutions are uniform!!!
+-- theorem DRWS.rel.substD_congr_uniform [USubstCongr R]
+--   {Γ Δ : Ctx? α} (σ : SubstDS φ Γ Δ) {A a b} {da : Δ ⊢ a : A} {db : Δ ⊢ b : A}
+--   (h : R.uniform.rel da db) : R.uniform.rel (da.substD σ) (db.substD σ)
+--   := by induction h generalizing Γ with
+--   | pos_unif hΔ hΔc hc hd ha hs hb hei hec hsb I =>
+--       apply substD_of_subst
+--       rename_i s Δ Δc Δl Δm Δr e e' A B X a b b' da ds db db'
+--       have _ : Δl.del := hΔc.left_del;
+--       let Γc := (σ.inLeft hΔ)
+--       let Γr := (σ.inRight hΔ)
+--       let hΓ : Γ.SSplit Γc Γr := (σ.ssplitIn hΔ)
+--       let σc : SubstDS φ Γc Δc := (σ.substLeft hΔ)
+--       let σr : SubstDS φ Γr Δr := (σ.substRight hΔ)
+--       have hcc : Γc.copy := sorry
+--       have hdd : Γc.del := sorry
+--       let Γl := (σc.inLeft hΔc)
+--       let Γm := (σc.inRight hΔc)
+--       have hΓc : Γc.SSplit Γl Γm := (σc.ssplitIn hΔc)
+--       have hllc : Δl.copy := hΔc.left_copy
+--       have hlcc : Γl.copy := sorry
+--       have hldd : Γl.del := sorry
+--       let ρcl : Γc.PWk Γm := hΓc.pwk_left_del
+--       let σl : SubstDS φ Γl Δl := (σc.substLeft hΔc)
+--       let σm : SubstDS φ Γm Δm := (σc.substRight hΔc)
+--       let dl := (ds.let₁ (hΔc.cons (.right _)) (db.wk1 _));
+--       let dr :=
+--           (db'.case (Δc.both.cons (.right _))
+--             Deriv.bv0.inl ((ds.pwk ((hΔc.pwk_left_del).scons _)).wk1 ⟨A, 0⟩).inr)
+--       simp only [Deriv.wk_let₁, Deriv.wk_iter] at *
+--       let daw := da.subst σr
+--       let dsw := ds.subst (σm.lift ⟨A, ⊤⟩)
+--       let dbw := (db.subst (σl.lift ⟨X, ⊤⟩))
+--       let dlw := dsw.let₁ (hΓc.cons (.right _)) (dbw.wk1 ⟨A, 0⟩)
+--       let dbw' := db'.subst (σc.lift ⟨A, ⊤⟩)
+--       let drw := dbw'.case (Γc.both.cons (.right _))
+--         Deriv.bv0.inl
+--         ((dsw.pwk (ρcl.scons _)).wk1 ⟨A, 0⟩).inr
+--       have hdlw : (s.subst (σm.lift ⟨A, ⊤⟩)).let₁ X
+--         (↑¹ (b.subst (σl.lift ⟨X , ⊤⟩))) = (s.let₁ X (↑¹ b)).subst (σc.lift ⟨A, ⊤⟩)
+--         := by sorry
+--       have hdrw :
+--         (b'.subst (σc.lift ⟨A, ⊤⟩)).case B A
+--           (inl B X (bv 0))
+--           (inr B X (↑¹ (s.subst (σm.lift ⟨A, ⊤⟩))))
+--         = subst (σc.lift ⟨A, ⊤⟩) (b'.case B A (inl B X (bv 0)) (inr B X (↑¹ s)))
+--         := by sorry
+--       have h : R.uniform.rel dlw drw := by
+--         convert
+--           Coherent.elim _ (dlw.cast_term hdlw) _ (drw.cast_term hdrw)
+--             (I (σc.lift ⟨A, ⊤⟩)).subst_of_substD using 1
+--         <;> simp [Deriv.cast_term, Deriv.cast]
+--       let dliw := Deriv.let₁ hΓ daw
+--                   (Deriv.iter (hΓc.cons (.right ⟨A, ⊤⟩))
+--                     inferInstance inferInstance
+--                     dsw (dbw.wk1 ⟨A, 0⟩))
+--       let driw := Deriv.iter hΓ inferInstance inferInstance daw dbw'
+--       have h : R.uniform.rel dliw driw := DRWS.uniform.pos_unif
+--         (ds := dsw) (da := daw) (db := dbw) (db' := dbw') hΓ hΓc
+--         inferInstance inferInstance inferInstance inferInstance inferInstance hei hec h
+--       have hliw : (ren ρr.ix a).let₁ A
+--                     ((ren (Ctx?.Wk.scons { ty := A, q := ⊤ } ρm).ix s).iter X B
+--                       (ren (↑ⁿ Nat.succ) (ren (Ctx?.Wk.scons { ty := X, q := ⊤ } ρl).ix b))) =
+--                   (ren ρ.ix (a.let₁ A (s.iter X B (ren (↑ⁿ Nat.succ) b)))) := by
+--                   simp only [
+--                     Ctx?.Wk.ix, ren, ren_ren, <-Nat.liftWk_comp, Nat.liftWk_comp_succ,
+--                     ρci, ρli, ρmi, ρri
+--                   ]
+--       have hriw : (ren ρr.ix a).iter A B (ren (Ctx?.Wk.scons { ty := A, q := ⊤ } ρc).ix b')
+--                   = (ren ρ.ix (a.iter A B b')) := by simp [ρri, ρci]
+--       exact Coherent.elim
+--         (dliw.cast_term hliw) _ (driw.cast_term hriw) _
+--         (h.cast_term hliw hriw)
+--   | neg_unif hΔ hΔc hc hd ha hs hb hei hec hsb I => sorry
+--   | base => apply rel.of_cast_term; apply USubstCongr.usubst_congr; assumption
+--   | refl =>  apply rel.substD_of_subst; apply uniform.refl
+--   | trans => apply uniform.trans <;> apply_assumption
+--   | _ => stop simp only [Deriv.substD]; constructor <;> apply_assumption
