Refinery/Term/Extrinsic/Wf/PreBeta.lean
@@ -12,11 +12,10 @@ variable  {φ : Type u} {α : Type v} {ε : Type w} [S : Signature φ α ε]
           {R : DRWS φ α}
 
 theorem Wf.pre_beta_pos  {Γ Γl Γr : Ctx? α} {A : Ty α}
-    (hΓ : Γ.SSplit Γl Γr) (a : Wf R Γr A) (q : Quant) (hq : q ≤ quant Γr)
-    (b : Wf R (Γl.cons ⟨A, q⟩) B)
-    {el er} [ha : HasEff el a.tm] [hb : HasEff er b.tm] (he : el ⇀ er) (heq : q ≤ (pquant el).pos)
-    : a.let₁ hΓ (b.pwk ((Ctx?.PWk.refl Γl).cons (by simp)))
-    ≤ b.subst (SubstDS.subst0 hΓ a.deriv q hq)
+  (hΓ : Γ.SSplit Γl Γr) (a : Wf R Γr A) (q : Quant) (hq : q ≤ quant Γr)
+  (b : Wf R (Γl.cons ⟨A, q⟩) B)
+  {el er} [ha : HasEff el a.tm] [hb : HasEff er b.tm] (he : el ⇀ er) (heq : q ≤ (pquant el).pos)
+  : a.let₁ hΓ (b.pwk ((Ctx?.PWk.refl Γl).cons (by simp))) ≤ b.subst (SubstDS.subst0 hΓ a.deriv q hq)
     := by
     apply DRWS.uniform.base
     apply DRWS.refStep.beta
@@ -64,3 +63,28 @@ theorem Wf.pre_beta_pureLout {Γ Γl Γr : Ctx? α} {A : Ty α}
     : a.let₁ hΓ (b.pwk ((Ctx?.PWk.refl Γl).cons (by simp)))
     ≈ b.subst (SubstDS.subst0 hΓ a.deriv 1 bot_le)
     := pre_beta hΓ a 1 bot_le b (commutes_bot_right (l := ⊤)) bot_le
+
+theorem Wf.let₁_eta_pwk {Γ Γl Γr : Ctx? α}
+  {A : Ty α} (a : Wf R Γr A) (hΓ : Γ.SSplit Γl Γr) [hΓl : Γl.del]
+  : a.let₁ hΓ .bv0 ≈ a.pwk (hΓ.pwk_left_del) := by
+  apply (Wf.pre_beta_pureLout hΓ a .bv0 (hb := by simp [bv0])).coh <;> rfl
+
+theorem Wf.let₁_eta' {Γ : Ctx? α} {A : Ty α}
+  (a : Wf R Γ A) (hΓ : Γ.SSplit Γl Γ) [hΓl : Γl.del] : a.let₁ hΓ .bv0 ≈ a := by
+  apply (Wf.pre_beta_pureLout hΓ a .bv0 (hb := by simp [bv0])).coh <;> rfl
+
+theorem Wf.let₁_eta {Γ : Ctx? α} {A : Ty α} (a : Wf R Γ A) : a.let₁ Γ.erase_left .bv0 ≈ a
+:= a.let₁_eta' _
+
+theorem Eqv.let₁_eta_pwk [R.UWkCongr] {Γ Γl Γr : Ctx? α}
+  {A : Ty α} (a : Eqv R Γr A) (hΓ : Γ.SSplit Γl Γr) [hΓl : Γl.del]
+  : a.let₁ hΓ .bv0 = a.pwk (hΓ.pwk_left_del) := by
+  induction a using Eqv.quotInd; apply sound; apply Wf.let₁_eta_pwk
+
+theorem Eqv.let₁_eta'
+  {Γ : Ctx? α} {A : Ty α} (a : Eqv R Γ A) (hΓ : Γ.SSplit Γl Γ) [hΓl : Γl.del]
+  : a.let₁ hΓ .bv0 = a := by
+  induction a using Eqv.quotInd; apply sound; apply Wf.let₁_eta'
+
+theorem Eqv.let₁_eta {Γ : Ctx? α} {A : Ty α} (a : Eqv R Γ A) : a.let₁ Γ.erase_left .bv0 = a := by
+  induction a using Eqv.quotInd; apply sound; apply Wf.let₁_eta
